Add `--no-shiftr-avoid-uint1`
We now default to avoiding uint1 in the result of `>>` operations, as
per
https://github.com/mit-plv/fiat-crypto/pull/1015#discussion_r708691741.

This is required for making symbolic equivalence checking with assembly
go through.  It might be possible to improve the symbolic equivalence
checker to know enough about bounds analysis (or to also do bounds
analysis) so that this is not necessary?

src/AbstractInterpretation/AbstractInterpretation.v
@@ -409,10 +409,10 @@ Module Compilers.
              | _ => fun _ => None
              end%option%etype.
 
-        Definition abstract_interp_ident (assume_cast_truncates : bool) t (idc : ident t) : type.interp abstract_domain' t
+        Definition abstract_interp_ident {opts : AbstractInterpretation.Options} (assume_cast_truncates : bool) t (idc : ident t) : type.interp abstract_domain' t
           := ZRange.ident.option.interp assume_cast_truncates idc.
 
-        Definition always_strip_annotation (assume_cast_truncates : bool) {var} t (idc : ident t) : option (value var t)
+        Definition always_strip_annotation {opts : AbstractInterpretation.Options} (assume_cast_truncates : bool) {var} t (idc : ident t) : option (value var t)
           := match idc in ident t return option (value var t) with
              | ident.Z_cast as idc
              | ident.Z_cast2 as idc
@@ -437,7 +437,7 @@ Module Compilers.
              | _ => None
              end.
 
-        Definition strip_annotation (assume_cast_truncates : bool) (strip_annotations : bool) {var} : forall t, ident t -> option (value var t)
+        Definition strip_annotation {opts : AbstractInterpretation.Options} (assume_cast_truncates : bool) (strip_annotations : bool) {var} : forall t, ident t -> option (value var t)
           := if strip_annotations
              then always_strip_annotation assume_cast_truncates
              else fun _ _ => None.
@@ -485,47 +485,48 @@ Module Compilers.
         Definition strip_all_annotations strip_annotations_under {var} {t} (e : @expr var t) : @expr var t
           := @ident.strip_all_annotations var (@annotation_to_cast _) strip_annotations_under t e.
 
-        Definition eval_with_bound (assume_cast_truncates : bool) (skip_annotations_under : forall t, ident t -> bool) (strip_preexisting_annotations : bool) {var} {t} (e : @expr _ t) (bound : type.for_each_lhs_of_arrow abstract_domain t) : expr t
+        Definition eval_with_bound {opts : AbstractInterpretation.Options} (assume_cast_truncates : bool) (skip_annotations_under : forall t, ident t -> bool) (strip_preexisting_annotations : bool) {var} {t} (e : @expr _ t) (bound : type.for_each_lhs_of_arrow abstract_domain t) : expr t
           := let annotate_with_state := true in
              (@partial.ident.eval_with_bound)
                var abstract_domain' annotate_expr bottom' (abstract_interp_ident assume_cast_truncates) extract_list_state extract_option_state is_annotated_for (strip_annotation assume_cast_truncates strip_preexisting_annotations) skip_annotations_under annotate_with_state t e bound.
 
         Definition eta_expand_with_bound {var} {t} (e : @expr _ t) (bound : type.for_each_lhs_of_arrow abstract_domain t) : expr t
           := let assume_cast_truncates := false in
+             let shiftr_avoid_uint1 : shiftr_avoid_uint1_opt := false (* this doesn't actually matter for [eta_expand_with_bound], which only invokes [abstract_interp_ident] on things like [fst], [snd], etc *) in
              (@partial.ident.eta_expand_with_bound)
                var abstract_domain' annotate_expr bottom' (abstract_interp_ident assume_cast_truncates) extract_list_state extract_option_state is_annotated_for t e bound.
 
         Definition StripAllAnnotations strip_annotations_under {t} (e : Expr t) : Expr t
           := fun var => strip_all_annotations strip_annotations_under (e _).
 
-        Definition EvalWithBound (assume_cast_truncates : bool) (skip_annotations_under : forall t, ident t -> bool) (strip_preexisting_annotations : bool) {t} (e : Expr t) (bound : type.for_each_lhs_of_arrow abstract_domain t) : Expr t
+        Definition EvalWithBound {opts : AbstractInterpretation.Options} (assume_cast_truncates : bool) (skip_annotations_under : forall t, ident t -> bool) (strip_preexisting_annotations : bool) {t} (e : Expr t) (bound : type.for_each_lhs_of_arrow abstract_domain t) : Expr t
           := fun var => eval_with_bound assume_cast_truncates skip_annotations_under strip_preexisting_annotations (e _) bound.
         Definition EtaExpandWithBound {t} (e : Expr t) (bound : type.for_each_lhs_of_arrow abstract_domain t) : Expr t
           := fun var => eta_expand_with_bound (e _) bound.
       End with_relax.
 
-      Definition strip_annotations (assume_cast_truncates : bool) {var} {t} (e : @expr _ t) (bound : type.for_each_lhs_of_arrow abstract_domain t) : expr t
+      Definition strip_annotations {opts : AbstractInterpretation.Options} (assume_cast_truncates : bool) {var} {t} (e : @expr _ t) (bound : type.for_each_lhs_of_arrow abstract_domain t) : expr t
         := let strip_preexisting_annotations := true in
            let annotate_with_state := false in
            let skip_annotations_under := fun _ _ => false in
            (@partial.ident.eval_with_bound)
              var abstract_domain' (annotate_expr default_relax_zrange) bottom' (abstract_interp_ident assume_cast_truncates) extract_list_state extract_option_state (is_annotated_for default_relax_zrange) (strip_annotation assume_cast_truncates strip_preexisting_annotations) skip_annotations_under annotate_with_state t e bound.
 
-      Definition StripAnnotations (assume_cast_truncates : bool) {t} (e : Expr t) (bound : type.for_each_lhs_of_arrow abstract_domain t) : Expr t
+      Definition StripAnnotations {opts : AbstractInterpretation.Options} (assume_cast_truncates : bool) {t} (e : Expr t) (bound : type.for_each_lhs_of_arrow abstract_domain t) : Expr t
         := fun var => strip_annotations assume_cast_truncates (e _) bound.
 
-      Definition eval {var} {t} (e : @expr _ t) : expr t
+      Definition eval {opts : AbstractInterpretation.Options} {var} {t} (e : @expr _ t) : expr t
         := let assume_cast_truncates := false in
            let strip_preexisting_annotations := false in
            (@partial.ident.eval)
              var abstract_domain' (annotate_expr default_relax_zrange) bottom' (abstract_interp_ident assume_cast_truncates) extract_list_state extract_option_state (is_annotated_for default_relax_zrange) (strip_annotation assume_cast_truncates strip_preexisting_annotations)  t e.
-      Definition Eval {t} (e : Expr t) : Expr t
+      Definition Eval {opts : AbstractInterpretation.Options} {t} (e : Expr t) : Expr t
         := fun var => eval (e _).
       Definition EtaExpandWithListInfoFromBound {t} (e : Expr t) (bound : type.for_each_lhs_of_arrow abstract_domain t) : Expr t
         := EtaExpandWithBound default_relax_zrange e (type.map_for_each_lhs_of_arrow (@ZRange.type.option.strip_ranges) bound).
-      Definition extract (assume_cast_truncates : bool) {t} (e : expr t) (bound : type.for_each_lhs_of_arrow abstract_domain t) : abstract_domain' (type.final_codomain t)
+      Definition extract {opts : AbstractInterpretation.Options} (assume_cast_truncates : bool) {t} (e : expr t) (bound : type.for_each_lhs_of_arrow abstract_domain t) : abstract_domain' (type.final_codomain t)
         := @partial.ident.extract abstract_domain' bottom' (abstract_interp_ident assume_cast_truncates) t e bound.
-      Definition Extract (assume_cast_truncates : bool) {t} (e : Expr t) (bound : type.for_each_lhs_of_arrow abstract_domain t) : abstract_domain' (type.final_codomain t)
+      Definition Extract {opts : AbstractInterpretation.Options} (assume_cast_truncates : bool) {t} (e : Expr t) (bound : type.for_each_lhs_of_arrow abstract_domain t) : abstract_domain' (type.final_codomain t)
         := @partial.ident.extract abstract_domain' bottom' (abstract_interp_ident assume_cast_truncates) t (e _) bound.
     End specialized.
   End partial.
@@ -550,6 +551,7 @@ Module Compilers.
   End CheckCasts.
 
   Definition PartialEvaluateWithBounds
+             {shiftr_avoid_uint1 : shiftr_avoid_uint1_opt}
              (relax_zrange : zrange -> option zrange)
              (assume_cast_truncates : bool)
              (skip_annotations_under : forall t, ident t -> bool)
@@ -558,12 +560,15 @@ Module Compilers.
              (bound : type.for_each_lhs_of_arrow ZRange.type.option.interp t)
     : Expr t
     := partial.EvalWithBound relax_zrange assume_cast_truncates skip_annotations_under strip_preexisting_annotations (GeneralizeVar.GeneralizeVar (e _)) bound.
-  Definition PartialEvaluateWithListInfoFromBounds {t} (e : Expr t)
+  Definition PartialEvaluateWithListInfoFromBounds
+             {shiftr_avoid_uint1 : shiftr_avoid_uint1_opt}
+             {t} (e : Expr t)
              (bound : type.for_each_lhs_of_arrow ZRange.type.option.interp t)
     : Expr t
     := partial.EtaExpandWithListInfoFromBound (GeneralizeVar.GeneralizeVar (e _)) bound.
 
   Definition CheckedPartialEvaluateWithBounds
+             {shiftr_avoid_uint1 : shiftr_avoid_uint1_opt}
              (relax_zrange : zrange -> option zrange)
              (assume_cast_truncates : bool)
              (skip_annotations_under : forall t, ident t -> bool)
