src/CLI.v
@@ -316,6 +316,8 @@ Module ForExtraction.
         ["For any (comma-separated) bitwidths passed to this argument, use bitwidth-sized bounds rather than tighter bounds for the carry return value of primitives such as addcarryx and subborrowx."]).
   Definition cmovznz_by_mul_spec : named_argT
     := ([Arg.long_key "cmovznz-by-mul"], Arg.Unit, ["Use an alternative implementation of cmovznz using multiplication rather than bitwise-and with -1."]).
+  Definition no_shiftr_avoid_uint1_spec : named_argT
+    := ([Arg.long_key "no-shiftr-avoid-uint1"], Arg.Unit, ["Don't avoid uint1 types at the output of (>>) operations."]).
   Definition tight_bounds_multiplier_default := default_tight_upperbound_fraction.
   Definition tight_bounds_multiplier_spec : named_argT
     := ([Arg.long_key "tight-bounds-mul-by"],
@@ -473,6 +475,9 @@ Module ForExtraction.
       ; output_options :> output_options_opt
       (** Should we use the alternate implementation of cmovznz *)
       ; use_mul_for_cmovznz :> use_mul_for_cmovznz_opt
+      (** Various abstract interpretation options *)
+      (** Should we avoid uint1 at the output of shiftr *)
+      ; abstract_interpretation_options :> AbstractInterpretation.Options
       (** Should we split apart oversized operations? *)
       ; should_split_mul :> should_split_mul_opt
       (** Should we split apart multi-return operations? *)
@@ -574,6 +579,7 @@ Module ForExtraction.
         ; no_field_element_typedefs_spec
         ; relax_primitive_carry_to_bitwidth_spec
         ; cmovznz_by_mul_spec
+        ; no_shiftr_avoid_uint1_spec
         ; only_signed_spec
         ; hint_file_spec
         ; output_file_spec
@@ -620,6 +626,7 @@ Module ForExtraction.
              , no_field_element_typedefsv
              , relax_primitive_carry_to_bitwidthv
              , cmovznz_by_mulv
+             , no_shiftr_avoid_uint1v
              , only_signedv
              , hint_file_namesv
              , output_file_namev
@@ -682,6 +689,9 @@ Module ForExtraction.
                   ; should_split_multiret := to_bool split_multiretv
                   ; unfold_value_barrier := negb (to_bool value_barrierv)
                   ; use_mul_for_cmovznz := to_bool cmovznz_by_mulv
+                  ; abstract_interpretation_options :=
+                      {| AbstractInterpretation.shiftr_avoid_uint1 := negb (to_bool no_shiftr_avoid_uint1v)
+                      |}
                   ; emit_primitives := negb (to_bool no_primitivesv)
                   ; output_options :=
                       {| skip_typedefs_ := to_bool no_field_element_typedefsv
