src/PushButtonSynthesis/BarrettReduction.v
@@ -64,6 +64,7 @@ Section rbarrett_red.
   Local Existing Instance default_language_naming_conventions.
   Local Existing Instance default_documentation_options.
   Local Existing Instance default_output_options.
+  Local Existing Instance AbstractInterpretation.default_Options.
   Local Instance widen_carry : widen_carry_opt := false.
   Local Instance widen_bytes : widen_bytes_opt := true.
   Local Instance only_signed : only_signed_opt := false.
