src/Stringification/Rust.v
@@ -386,6 +386,7 @@ Module Rust.
   Local Instance : lift_declarations_opt := false.
 
   Definition ToFunctionLines
+             {absint_opts : AbstractInterpretation.Options}
              {relax_zrange : relax_zrange_opt}
              {language_naming_conventions : language_naming_conventions_opt}
              {documentation_options : documentation_options_opt}
